coq-SystemRF-1.1/Denotations/BasicPropsCSubst.v
@@ -1,10 +1,10 @@
 Require Import SystemRF.BasicDefinitions.
 Require Import SystemRF.Names.
-(*Require Import SystemRF.Semantics.
+Require Import SystemRF.Strengthenings.
 Require Import SystemRF.SystemFTyping.
-Require Import SystemRF.WellFormedness.*)
+Require Import SystemRF.WellFormedness.
 Require Import SystemRF.BasicPropsSubstitution.
-(*Require Import SystemRF.BasicPropsEnvironments.*)
+Require Import SystemRF.BasicPropsEnvironments.
 Require Import Denotations.ClosingSubstitutions.
 
 Require Import Arith.
@@ -12,282 +12,254 @@ Require Import Arith.
   (* -- | More Properties of Substitution *)
 
 Lemma lem_commute_subFV : (forall (e:expr) (x:vname) (v:expr) (y:vname) (v_y:expr),
-    y <> x -> ~ Elem x (fv v_y)
-      -> subFV y v_y (subFV x v e) = subFV x (subFV y v_y v) (subFV y v_y e) ) * ((
+    y <> x -> ~ Elem x (fv v_y) -> ~ Elem y (fv v)
+      -> subFV y v_y (subFV x v e) = subFV x v (subFV y v_y e) ) * ((
   forall (t:type) (x:vname) (v:expr) (y:vname) (v_y:expr),
-    y <> x -> ~ Elem x (fv v_y)
-      -> tsubFV y v_y (tsubFV x v t) = tsubFV x (subFV y v_y v) (tsubFV y v_y t) ) * (
+    y <> x -> ~ Elem x (fv v_y) -> ~ Elem y (fv v)
+      -> tsubFV y v_y (tsubFV x v t) = tsubFV x v (tsubFV y v_y t) ) * (
   forall (ps:preds) (x:vname) (v:expr) (y:vname) (v_y:expr),
-    y <> x -> ~ Elem x (fv v_y)
-      -> psubFV y v_y (psubFV x v ps) = psubFV x (subFV y v_y v) (psubFV y v_y ps) )).
+    y <> x -> ~ Elem x (fv v_y) -> ~ Elem y (fv v)
+      -> psubFV y v_y (psubFV x v ps) = psubFV x v (psubFV y v_y ps) )).
 Proof. apply ( syntax_mutind
   (fun e : expr => forall (x:vname) (v:expr) (y:vname) (v_y:expr),
-    y <> x -> ~ Elem x (fv v_y)
-      -> subFV y v_y (subFV x v e) = subFV x (subFV y v_y v) (subFV y v_y e) )
+    y <> x -> ~ Elem x (fv v_y) -> ~ Elem y (fv v)
+      -> subFV y v_y (subFV x v e) = subFV x v (subFV y v_y e) )
   (fun t : type => forall (x:vname) (v:expr) (y:vname) (v_y:expr),
-    y <> x -> ~ Elem x (fv v_y)
-      -> tsubFV y v_y (tsubFV x v t) = tsubFV x (subFV y v_y v) (tsubFV y v_y t) )
+    y <> x -> ~ Elem x (fv v_y) -> ~ Elem y (fv v)
+      -> tsubFV y v_y (tsubFV x v t) = tsubFV x v (tsubFV y v_y t) )
   (fun ps : preds => forall (x:vname) (v:expr) (y:vname) (v_y:expr),
-    y <> x -> ~ Elem x (fv v_y)
-      -> psubFV y v_y (psubFV x v ps) = psubFV x (subFV y v_y v) (psubFV y v_y ps) ))
+    y <> x -> ~ Elem x (fv v_y) -> ~ Elem y (fv v)
+      -> psubFV y v_y (psubFV x v ps) = psubFV x v (psubFV y v_y ps) ))
   ; intros; simpl; try reflexivity
   ; (* 1 IH *) try ( apply f_equal; apply H; assumption)
   ; (* 2 IH *) try ( apply f_equal2; apply H || apply H0; assumption ).
   - (* FV *) destruct (Nat.eqb x0 x) eqn:E0; 
     destruct (Nat.eqb y x) eqn:E; simpl;
-    try rewrite E0; try rewrite E;
-    try reflexivity; try symmetry;
+    try rewrite E0; try rewrite E; try reflexivity;
     (* both E0 and E cannot be true *)
     try apply Nat.eqb_eq in E0; try apply Nat.eqb_eq in E;
-    try rewrite E0 in H; try rewrite E in H; try contradiction.
-    apply lem_subFV_notin; assumption.
+    try rewrite E0 in H; try rewrite E in H; try contradiction;
+    apply lem_subFV_notin || (symmetry; apply lem_subFV_notin); assumption.
   - (* If *) rewrite H; try rewrite H0; try rewrite H1; trivial.
   Qed.
 
-(*Definition closed (e : expr) := fv e = empty /\ ftv e = empty.*)
+Lemma lem_commute_subFV_subFTV : (forall (e:expr) (a:vname) (t_a:type) (y:vname) (v_y:expr),
+    noExists t_a -> isValue v_y -> ~ Elem a (ftv v_y) -> ~ Elem y (free t_a)
+      -> subFV y v_y (subFTV a t_a e) = subFTV a t_a (subFV y v_y e) ) * ((
+  forall (t:type) (a:vname) (t_a:type) (y:vname) (v_y:expr),
+    noExists t_a -> isValue v_y -> ~ Elem a (ftv v_y) -> ~ Elem y (free t_a)
+      -> tsubFV y v_y (tsubFTV a t_a t) = tsubFTV a t_a (tsubFV y v_y t) ) * (
+  forall (ps:preds) (a:vname) (t_a:type) (y:vname) (v_y:expr),
+    noExists t_a -> isValue v_y -> ~ Elem a (ftv v_y) -> ~ Elem y (free t_a)
+      -> psubFV y v_y (psubFTV a t_a ps) = psubFTV a t_a (psubFV y v_y ps) )).
+Proof. apply ( syntax_mutind
+  (fun e : expr => forall (a:vname) (t_a:type) (y:vname) (v_y:expr),
+    noExists t_a -> isValue v_y -> ~ Elem a (ftv v_y) -> ~ Elem y (free t_a)
+      -> subFV y v_y (subFTV a t_a e) = subFTV a t_a (subFV y v_y e) )
+  (fun t : type => forall (a:vname) (t_a:type) (y:vname) (v_y:expr),
+    noExists t_a -> isValue v_y -> ~ Elem a (ftv v_y) -> ~ Elem y (free t_a)
+      -> tsubFV y v_y (tsubFTV a t_a t) = tsubFTV a t_a (tsubFV y v_y t) )
+  (fun ps : preds => forall (a:vname) (t_a:type) (y:vname) (v_y:expr),
+    noExists t_a -> isValue v_y -> ~ Elem a (ftv v_y) -> ~ Elem y (free t_a)
+      -> psubFV y v_y (psubFTV a t_a ps) = psubFTV a t_a (psubFV y v_y ps) ))
+  ; intros; simpl; try reflexivity
+  ; (* 1 IH *) try ( apply f_equal; apply H; assumption)
+  ; (* 2 IH *) try ( apply f_equal2; apply H || apply H0; assumption ).
+  - (* FV *) destruct (Nat.eqb y x) eqn:E; simpl;
+    try rewrite E; try reflexivity;
+    symmetry; apply lem_subFTV_notin; assumption.
+  - (* If *) rewrite H; try rewrite H0; try rewrite H1; trivial.
+  - (* TRefn *) destruct b eqn:Eb; simpl; try rewrite H; trivial.
+    destruct (a =? a0); simpl; try rewrite lem_subFV_push;
+    try rewrite H; try f_equal; try apply lem_subFV_notin; trivial.
+  Qed. 
+
+Lemma lem_commute_subFTV : (
+  forall (e:expr) (a:vname) (t_a:type) (a':vname) (t_a':type),
+    noExists t_a -> noExists t_a' -> a' <> a 
+      -> ~ Elem a (freeTV t_a') -> ~ Elem a' (freeTV t_a)
+      -> subFTV a' t_a' (subFTV a t_a e) = subFTV a t_a (subFTV a' t_a' e) ) * ((
+  forall (t:type) (a:vname) (t_a:type) (a':vname) (t_a':type),
+    noExists t_a -> noExists t_a' -> a' <> a 
+      -> ~ Elem a (freeTV t_a') -> ~ Elem a' (freeTV t_a)
+      -> tsubFTV a' t_a' (tsubFTV a t_a t) = tsubFTV a t_a (tsubFTV a' t_a' t) ) * (
+  forall (ps:preds) (a:vname) (t_a:type) (a':vname) (t_a':type),
+    noExists t_a -> noExists t_a' -> a' <> a 
+      -> ~ Elem a (freeTV t_a') -> ~ Elem a' (freeTV t_a)
+      -> psubFTV a' t_a' (psubFTV a t_a ps) = psubFTV a t_a (psubFTV a' t_a' ps) )).
+Proof. apply ( syntax_mutind
+  (fun e : expr => forall (a:vname) (t_a:type) (a':vname) (t_a':type),
+    noExists t_a -> noExists t_a' -> a' <> a 
+      -> ~ Elem a (freeTV t_a') -> ~ Elem a' (freeTV t_a)
+      -> subFTV a' t_a' (subFTV a t_a e) = subFTV a t_a (subFTV a' t_a' e) )
+  (fun t : type => forall (a:vname) (t_a:type) (a':vname) (t_a':type),
+    noExists t_a -> noExists t_a' -> a' <> a 
+      -> ~ Elem a (freeTV t_a') -> ~ Elem a' (freeTV t_a)
+      -> tsubFTV a' t_a' (tsubFTV a t_a t) = tsubFTV a t_a (tsubFTV a' t_a' t) )
+  (fun ps : preds => forall (a:vname) (t_a:type) (a':vname) (t_a':type),
+    noExists t_a -> noExists t_a' -> a' <> a 
+      -> ~ Elem a (freeTV t_a') -> ~ Elem a' (freeTV t_a)
+      -> psubFTV a' t_a' (psubFTV a t_a ps) = psubFTV a t_a (psubFTV a' t_a' ps) ))
+  ; intros; simpl; try reflexivity
+  ; (* 1 IH *) try ( apply f_equal; apply H; assumption)
+  ; (* 2 IH *) try ( apply f_equal2; apply H || apply H0; assumption ).
+  - (* If *) rewrite H; try rewrite H0; try rewrite H1; trivial.
+  - (* TRefn *) destruct b eqn:Eb; simpl; try rewrite H; trivial.
+    destruct (a =? a0) eqn:Ea; destruct (a' =? a0) eqn:Ea'; 
+    simpl; try rewrite Ea; try rewrite Ea';
+    (* both E0 and E cannot be true *)
+      try apply Nat.eqb_eq in Ea; try apply Nat.eqb_eq in Ea';
+      try rewrite Ea in H2; try rewrite Ea' in H2; try contradiction;
+    try rewrite lem_subFTV_push; try rewrite H; try f_equal;
+    try apply lem_subFTV_notin; try (symmetry; apply lem_subFTV_notin);
+    try subst a0; trivial.
+  Qed.
 
   (* -- | Closing Substitution Properties *)
 
-(*
 Lemma lem_unroll_csubst_left : forall (th:csub) (x:vname) (v_x e:expr),
-    ~ in_csubst x th -> (*isValue v_x ->*) fv v_x = empty /\ ftv v_x = empty
+    ~ in_csubst x th -> fv v_x = empty /\ ftv v_x = empty -> isValue v_x
+        -> closed th -> substitutable th
         -> csubst (CCons x v_x th) e = subFV x v_x (csubst th e).
 Proof. induction th; intros; simpl; try reflexivity;
   unfold in_csubst in H; simpl in H; 
   apply not_elem_names_add_elim in H; destruct H.
-  - rewrite <- IHth; simpl; try apply f_equal; 
-    try apply lem_commute_subFV; trivial. 
-    assert (subFV x v_x v_x0 = v_x0) by 
-      (apply lem_subFV_notin; destruct H0; rewrite H0; intuition).
-    rewrite <- H2 at 2. apply lem_commute_subFV.
+  - (* CCons *) rewrite <- IHth; simpl; try apply f_equal;
+    try apply lem_commute_subFV; 
+    simpl in H2; simpl in H3; try apply H0;
+    destruct H0; destruct H2; destruct H6; destruct H3;
+    try rewrite H0; try rewrite H2; intuition.
+  - (* CConsT *) rewrite <- IHth; simpl; try apply f_equal;
+    try symmetry; try apply lem_commute_subFV_subFTV;
+    simpl in H2; simpl in H3; try apply H0;
+    destruct H0; destruct H2; destruct H6; destruct H3;
+    try rewrite H2; try rewrite H5; intuition.
+  Qed.
     
-    assert (~ Elem x (fv v_x0)).
-    unfold closed in H0; destruct H0. rewrite H0. trivial. intuition.
-    
-    apply lem_com
-  
-  rewrite lem_commute_subFV.
+Lemma lem_unroll_ctsubst_left : forall (th:csub) (x:vname) (v_x:expr) (t:type),
+    ~ in_csubst x th -> fv v_x = empty /\ ftv v_x = empty -> isValue v_x
+        -> closed th -> substitutable th
+        -> ctsubst (CCons x v_x th) t = tsubFV x v_x (ctsubst th t).
+Proof. induction th; intros; simpl; try reflexivity;
+  unfold in_csubst in H; simpl in H; 
+  apply not_elem_names_add_elim in H; destruct H.
+  - (* CCons *) rewrite <- IHth; simpl; try apply f_equal;
+    try apply lem_commute_subFV; 
+    simpl in H2; simpl in H3; try apply H0;
+    destruct H0; destruct H2; destruct H6; destruct H3;
+    try rewrite H0; try rewrite H2; intuition.
+  - (* CConsT *) rewrite <- IHth; simpl; try apply f_equal;
+    try symmetry; try apply lem_commute_subFV_subFTV;
+    simpl in H2; simpl in H3; try apply H0;
+    destruct H0; destruct H2; destruct H6; destruct H3;
+    try rewrite H2; try rewrite H5; intuition.
+  Qed.       
 
-lem_unroll_csubst_left CEmpty           x v_x e = ()
-lem_unroll_csubst_left (CCons y v_y th) x v_x e 
-  = () ? lem_subFV_notin x v_x v_y
---             === ctsubst th (tsubFV y (subFV x v_x v_y) (tsubFV x v_x t))
-       ? lem_commute_subFV y v_y x v_x e
-{-             === ctsubst th (tsubFV x v_x (tsubFV y v_y t))
-               === ctsubst (CCons x v_x th) (tsubFV y v_y t)-}
-       ? lem_unroll_csubst_left th x v_x (subFV y v_y e)
-{-             === tsubFV x v_x (ctsubst th (tsubFV y v_y t))
-               === tsubFV x v_x (ctsubst (CCons y v_y th) t) )-}
-lem_unroll_csubst_left (CConsT a t_a th) x v_x e 
-  = () ? lem_tsubFV_notin x v_x t_a
-       ? lem_commute_subFV_subFTV a t_a x v_x e
-       ? lem_unroll_csubst_left th x v_x (subFTV a t_a e)
+Lemma lem_unroll_ctsubst_tv_left : forall (th:csub) (a:vname) (t_a t:type),
+    ~ in_csubst a th -> free t_a = empty /\ freeTV t_a = empty -> noExists t_a
+        -> closed th -> substitutable th
+        -> ctsubst (CConsT a t_a th) t = tsubFTV a t_a (ctsubst th t).
+Proof. induction th; intros; simpl; try reflexivity;
+  unfold in_csubst in H; simpl in H; 
+  apply not_elem_names_add_elim in H; destruct H.
+  - (* CCons *) rewrite <- IHth; simpl; try apply f_equal;
+    try apply lem_commute_subFV_subFTV;
+    simpl in H2; simpl in H3; try apply H0;
+    destruct H0; destruct H2; destruct H6; destruct H3;
+    try rewrite H0; try rewrite H6; intuition.
+  - (* CConsT *) rewrite <- IHth; simpl; try apply f_equal;
+    try symmetry; try apply lem_commute_subFTV;
+    simpl in H2; simpl in H3; try apply H0;
+    destruct H0; destruct H2; destruct H6; destruct H3;
+    try rewrite H5; try rewrite H6; intuition.
+  Qed.         
 
-{-@ lem_unroll_ctsubst_left :: th:CSub -> { x:Vname | not (in_csubst x th) } 
-        -> { v_x:Value | Set_emp (fv v_x) && Set_emp (ftv v_x) } ->  t:Type
-        -> { pf:_ | ctsubst (CCons x v_x th) t == tsubFV x v_x (ctsubst th t) } @-}
-lem_unroll_ctsubst_left :: CSub -> Vname -> Expr -> Type -> Proof
-lem_unroll_ctsubst_left CEmpty           x v_x t = ()
-lem_unroll_ctsubst_left (CCons y v_y th) x v_x t 
-  = () {-toProof ( ctsubst (CCons x v_x (CCons y v_y th)) t
-               === ctsubst (CCons y v_y th) (tsubFV x v_x t)
-               === ctsubst th (tsubFV y v_y (tsubFV x v_x t))-}
-                 ? lem_subFV_notin x v_x v_y
---             === ctsubst th (tsubFV y (subFV x v_x v_y) (tsubFV x v_x t))
-                 ? lem_commute_tsubFV y v_y x v_x t
-{-             === ctsubst th (tsubFV x v_x (tsubFV y v_y t))
-               === ctsubst (CCons x v_x th) (tsubFV y v_y t)-}
-                 ? lem_unroll_ctsubst_left th x v_x (tsubFV y v_y t)
-{-             === tsubFV x v_x (ctsubst th (tsubFV y v_y t))
-               === tsubFV x v_x (ctsubst (CCons y v_y th) t) )-}
-lem_unroll_ctsubst_left (CConsT a t_a th) x v_x t 
-  = () ? lem_tsubFV_notin x v_x t_a
-       ? lem_commute_tsubFV_tsubFTV a t_a x v_x t
-       ? lem_unroll_ctsubst_left th x v_x (tsubFTV a t_a t)
+  (* --- various distributive properties of csubst and ctsubst *)
 
-{-@ lem_unroll_ctsubst_tv_left :: th:CSub -> { a:Vname | not (in_csubst a th) } 
-        -> { t_a:UserType | Set_emp (free t_a) && Set_emp (freeTV t_a) } ->  t:Type
-        -> { pf:_ | ctsubst (CConsT a t_a th) t == tsubFTV a t_a (ctsubst th t) } @-}
-lem_unroll_ctsubst_tv_left :: CSub -> Vname -> Type -> Type -> Proof
-lem_unroll_ctsubst_tv_left CEmpty           a t_a t = ()
-lem_unroll_ctsubst_tv_left (CCons y v_y th) a t_a t
-  = () ? lem_tsubFV_notin  y v_y t_a
-       ? lem_commute_tsubFV_tsubFTV a t_a y v_y t
-       ? lem_unroll_ctsubst_tv_left th a t_a (tsubFV y v_y t)
-lem_unroll_ctsubst_tv_left (CConsT a' t' th) a t_a t
-  = () ? lem_tsubFTV_notin a' t' t_a
-       ? lem_commute_tsubFTV a t_a a' t' t
-       ? lem_unroll_ctsubst_tv_left th a t_a (tsubFTV a' t' t)
+Lemma lem_csubst_bc : forall (th:csub) (b:bool) ,
+    csubst th (Bc b) = Bc b.
+Proof. induction th; simpl; apply IHth || reflexivity. Qed.
 
-{-@ lem_in_csubst_concatCS :: th:CSub -> { th':CSub | Set_emp (Set_cap (bindsC th) (bindsC th')) }   
-      -> x:Vname -> {pf:_ | (in_csubst x (concatCS th th')) <=> ((in_csubst x th) || (in_csubst x th'))} @-} 
-lem_in_csubst_concatCS :: CSub -> CSub -> Vname -> Proof
-lem_in_csubst_concatCS th CEmpty          x = () 
-lem_in_csubst_concatCS th (CCons y v th') x = () ? lem_in_csubst_concatCS th th' x 
-lem_in_csubst_concatCS th (CConsT a t th') x = () ? lem_in_csubst_concatCS th th' x 
+Lemma lem_csubst_ic : forall (th:csub) (n:nat),
+    csubst th (Ic n) = Ic n.
+Proof. induction th; simpl; apply IHth || reflexivity. Qed.
 
-{-@ lem_binds_cons_concatCS :: th:CSub -> {  th':CSub | Set_emp (Set_cap (bindsC th) (bindsC th')) }
-      -> { x:Vname | not (Set_mem x (bindsC th)) && not (Set_mem x (bindsC th')) } 
-      -> { v_x:Value | Set_emp (fv v_x) && Set_emp (ftv v_x) }
-      -> { pf:_ | Set_sub (bindsC (concatCS th th')) (bindsC (concatCS (CCons x v_x th) th')) &&
-             bindsC (concatCS (CCons x v_x th) th') == Set_cup (Set_cup (bindsC th) (Set_sng x)) (bindsC th') } @-}
-lem_binds_cons_concatCS :: CSub -> CSub -> Vname -> Expr -> Proof
-lem_binds_cons_concatCS th CEmpty          x v_x = ()
-lem_binds_cons_concatCS th (CCons y s th') x v_x = () ? lem_binds_cons_concatCS th th' x v_x
-lem_binds_cons_concatCS th (CConsT a t th') x v_x = () ? lem_binds_cons_concatCS th th' x v_x
+Lemma lem_csubst_prim : forall (th:csub) (c:prim),
+    csubst th (Prim c) = Prim c.
+Proof. induction th; simpl; apply IHth || reflexivity. Qed.
 
-{-@ lem_binds_consT_concatCS :: th:CSub -> {  th':CSub | Set_emp (Set_cap (bindsC th) (bindsC th')) }
-      -> { a:Vname | not (Set_mem a (bindsC th)) && not (Set_mem a (bindsC th')) } 
-      -> { t_a:UserType | Set_emp (free t_a) && Set_emp (freeTV t_a) }
-      -> { pf:_ | Set_sub (bindsC (concatCS th th')) (bindsC (concatCS (CConsT a t_a th) th')) &&
-             bindsC (concatCS (CConsT a t_a th) th') == Set_cup (Set_cup (bindsC th) (Set_sng a)) (bindsC th') } @-}
-lem_binds_consT_concatCS :: CSub -> CSub -> Vname -> Type -> Proof
-lem_binds_consT_concatCS th CEmpty             a t_a = ()
-lem_binds_consT_concatCS th (CCons  y  s  th') a t_a = () ? lem_binds_consT_concatCS th th' a t_a
-lem_binds_consT_concatCS th (CConsT a' t' th') a t_a = () ? lem_binds_consT_concatCS th th' a t_a
+Lemma lem_csubst_bv : forall (th:csub) (y:vname),
+    csubst th (BV y) = BV y.
+Proof. induction th; simpl; apply IHth || reflexivity. Qed.
 
-  --- various distributive properties of csubst and ctsubst
+Lemma lem_csubst_fv : forall (th:csub) (y:vname),
+    ~ in_csubst y th -> csubst th (FV y) = FV y.
+Proof. induction th; unfold in_csubst; intros; simpl; 
+  simpl in H; try apply not_elem_names_add_elim in H; 
+  try destruct (x =? y) eqn:E;
+  try apply Nat.eqb_eq in E; try rewrite E in H;
+  try apply IHth; intuition. Qed.
 
-{-@ lem_csubst_bc :: th:CSub -> b:Bool -> { pf:_ | csubst th (Bc b) == Bc b } @-}
-lem_csubst_bc :: CSub -> Bool -> Proof
-lem_csubst_bc (CEmpty)       b = ()
-lem_csubst_bc (CCons x v th) b = () ? lem_csubst_bc th b
-lem_csubst_bc (CConsT a t th) b = () ? lem_csubst_bc th b
+Lemma lem_csubst_lambda : forall (th:csub) (e:expr),
+    csubst th (Lambda e) = Lambda (csubst th e).
+Proof. induction th; simpl; intro e; apply IHth || reflexivity. Qed.
 
-{-@ lem_csubst_ic :: th:CSub -> n:Int -> { pf:_ | csubst th (Ic n) == Ic n } @-}
-lem_csubst_ic :: CSub -> Int -> Proof
-lem_csubst_ic (CEmpty)       n = ()
-lem_csubst_ic (CCons x v th) n = () ? lem_csubst_ic th n
-lem_csubst_ic (CConsT a t th) n = () ? lem_csubst_ic th n
+Lemma lem_csubst_app : forall (th:csub) (e e':expr),
+    csubst th (App e e') = App (csubst th e) (csubst th e').
+Proof. induction th; simpl; intros e e'; apply IHth || reflexivity. Qed.
 
-{-@ lem_csubst_prim :: th:CSub -> c:Prim -> { pf:_ | csubst th (Prim c) == Prim c } @-}
-lem_csubst_prim :: CSub -> Prim -> Proof
-lem_csubst_prim (CEmpty)       c = ()
-lem_csubst_prim (CCons x v th) c = () ? lem_csubst_prim th c
-lem_csubst_prim (CConsT a t th) c = () ? lem_csubst_prim th c
+Lemma lem_csubst_lambdaT : forall (th:csub) (k:kind) (e:expr),
+    csubst th (LambdaT k e) = LambdaT k (csubst th e).
+Proof. induction th; simpl; intros k e; apply IHth || reflexivity. Qed.
 
-{-@ lem_csubst_bv :: th:CSub -> y:Vname -> { pf:_ | csubst th (BV y) == BV y } @-}
-lem_csubst_bv :: CSub -> Vname -> Proof
-lem_csubst_bv (CEmpty)       y = ()
-lem_csubst_bv (CCons x v th) y = () ? lem_csubst_bv th y
-lem_csubst_bv (CConsT a t th) y = () ? lem_csubst_bv th y
+Lemma lem_csubst_appT : forall (th:csub) (e:expr) (t:type),
+    csubst th (AppT e t) = AppT (csubst th e) (ctsubst th t).
+Proof. induction th; simpl; intros; apply IHth || reflexivity. Qed.
+ 
+Lemma lem_csubst_let : forall (th:csub) (e_x e:expr), 
+    csubst th (Let e_x e) = Let (csubst th e_x) (csubst th e).
+Proof. induction th; simpl; intros; apply IHth || reflexivity. Qed.
 
-{-@ lem_csubst_fv :: th:CSub -> { y:Vname | not (in_csubst y th) } -> { pf:_ | csubst th (FV y) == FV y } @-} 
-lem_csubst_fv :: CSub -> Vname -> Proof
-lem_csubst_fv (CEmpty)        y = ()
-lem_csubst_fv (CCons x v th)  y = () ? lem_csubst_fv th y 
-lem_csubst_fv (CConsT a t th) y = () ? lem_csubst_fv th y 
+Lemma lem_csubst_annot : forall (th:csub) (e:expr) (t:type),
+    csubst th (Annot e t) = Annot (csubst th e) (ctsubst th t).
+Proof. induction th; simpl; intros; apply IHth || reflexivity. Qed.
 
-{-@ lem_csubst_lambda :: th:CSub -> x:Vname 
-        -> e:Expr -> { pf:_ | csubst th (Lambda x e) == Lambda x (csubst th e) } @-}
-lem_csubst_lambda :: CSub -> Vname -> Expr -> Proof
-lem_csubst_lambda (CEmpty)        x e = ()
-lem_csubst_lambda (CCons y v th)  x e = () ? lem_csubst_lambda th x (subFV y v e)
-lem_csubst_lambda (CConsT a t th) x e = () ? lem_csubst_lambda th x (subFTV a t e)
+Lemma lem_csubst_if : forall (th:csub) (e0 e1 e2:expr), 
+    csubst th (If e0 e1 e2) = If (csubst th e0) (csubst th e1) (csubst th e2).
+Proof. induction th; simpl; intros; apply IHth || reflexivity. Qed.
 
-{-@ lem_csubst_app :: th:CSub -> e:Expr -> e':Expr 
-               -> { pf:_ | csubst th (App e e') == App (csubst th e) (csubst th e') } @-}
-lem_csubst_app :: CSub -> Expr -> Expr -> Proof
-lem_csubst_app (CEmpty)        e e' = ()
-lem_csubst_app (CCons y v th)  e e' = () ? lem_csubst_app th (subFV y v e) (subFV y v e')
-lem_csubst_app (CConsT a t th) e e' = () ? lem_csubst_app th (subFTV a t e) (subFTV a t e')
+Lemma lem_cpsubst_pempty : forall (th:csub), cpsubst th PEmpty = PEmpty.
+Proof. induction th; simpl; apply IHth || reflexivity. Qed.
 
-{-@ lem_csubst_lambdaT :: th:CSub -> a:Vname -> k:Kind
-        -> e:Expr -> { pf:_ | csubst th (LambdaT a k e) == LambdaT a k (csubst th e) } @-}
-lem_csubst_lambdaT :: CSub -> Vname -> Kind -> Expr -> Proof
-lem_csubst_lambdaT (CEmpty)         a k e = ()
-lem_csubst_lambdaT (CCons y v th)   a k e = () ? lem_csubst_lambdaT th a k (subFV y v e)
-lem_csubst_lambdaT (CConsT a1 t th) a k e = () ? lem_csubst_lambdaT th a k (subFTV a1 t e)
+Lemma lem_cpsubst_pcons : forall (th:csub) (p:expr) (ps:preds),
+    cpsubst th (PCons p ps) = PCons (csubst th p) (cpsubst th ps).
+Proof. induction th; simpl; intros; apply IHth || reflexivity. Qed.
+ 
+Lemma lem_cpsubst_strengthen : forall (th:csub) (ps qs:preds),
+    cpsubst th (strengthen ps qs) = strengthen (cpsubst th ps) (cpsubst th qs).
+Proof. induction th; simpl; intros; 
+  try rewrite lem_psubFV_strengthen; try rewrite lem_psubFTV_strengthen; 
+  try apply IHth || reflexivity. Qed.
 
-{-@ lem_csubst_appT :: th:CSub -> e:Expr -> t:UserType
-        -> { pf:_ | csubst th (AppT e t) == AppT (csubst th e) (ctsubst th t) } @-}
-lem_csubst_appT :: CSub -> Expr -> Type -> Proof
-lem_csubst_appT (CEmpty)          e t = ()
-lem_csubst_appT (CCons y v th)    e t = () ? lem_csubst_appT th (subFV y v e)    (tsubFV y v t)
-lem_csubst_appT (CConsT a t_a th) e t = () ? lem_csubst_appT th (subFTV a t_a e) (tsubFTV a t_a t)
+Lemma lem_ctsubst_push : forall (th:csub) (ps:preds) (t_a:type),
+    noExists t_a -> substitutable th
+        -> ctsubst th (push ps t_a) = push (cpsubst th ps) (ctsubst th t_a).
+Proof. induction th; simpl; intros;
+  try rewrite lem_subFV_push; try rewrite lem_subFTV_push;
+  try rewrite IHth; 
+  try apply lemma_tsubFV_noExists; try apply lemma_tsubFTV_noExists;
+  intuition. Qed.
 
-{-@ lem_csubst_let :: th:CSub -> x:Vname -> e_x:Expr -> e:Expr 
-        -> { pf:_ | csubst th (Let x e_x e) == Let x (csubst th e_x) (csubst th e) } @-}
-lem_csubst_let :: CSub -> Vname -> Expr -> Expr -> Proof
-lem_csubst_let (CEmpty)       x e_x e  = ()
-lem_csubst_let (CCons y v th) x e_x e  = () ? lem_csubst_let th x (subFV y v e_x) (subFV y v e)
-lem_csubst_let (CConsT a t th) x e_x e = () ? lem_csubst_let th x (subFTV a t e_x) (subFTV a t e)
-
-{-@ lem_csubst_annot :: th:CSub -> e:Expr
-        -> t:UserType -> { pf:_ | csubst th (Annot e t) == Annot (csubst th e) (ctsubst th t) } @-}
-lem_csubst_annot :: CSub -> Expr -> Type -> Proof
-lem_csubst_annot (CEmpty)       e t    = ()
-lem_csubst_annot (CCons y v th) e t    = () ? lem_csubst_annot th (subFV y v e) (tsubFV y v t)
-lem_csubst_annot (CConsT a t_a th) e t = () ? lem_csubst_annot th (subFTV a t_a e) (tsubFTV a t_a t)
-
-{-@ lem_csubst_conj :: th:CSub -> e:Expr -> e':Expr 
-               -> { pf:_ | csubst th (Conj e e') == Conj (csubst th e) (csubst th e') } @-}
-lem_csubst_conj :: CSub -> Expr -> Expr -> Proof
-lem_csubst_conj (CEmpty)        e e' = ()
-lem_csubst_conj (CCons y v th)  e e' = () ? lem_csubst_conj th (subFV y v e) (subFV y v e')
-lem_csubst_conj (CConsT a t th) e e' = () ? lem_csubst_conj th (subFTV a t e) (subFTV a t e')
-
-{-@ lem_csubst_trivial :: th:CSub -> { tt:Pred | isTrivial tt } -> { pf:_ | csubst th tt == tt } @-}
-lem_csubst_trivial :: CSub -> Expr -> Proof
-lem_csubst_trivial th (Bc True) = () ? lem_csubst_bc th True
-lem_csubst_trivial th (Conj p r) = case p of
-  (Bc True) -> () ? lem_csubst_conj th (Bc True) r
-                  ? lem_csubst_bc th  True
-                  ? lem_csubst_trivial th r
-{-
-{-@ lem_csubst_conjunction :: th:CSub -> { p:Pred | not (isConjunction p) }
-        -> { pf:_ | not (isConjunction (csubst th p)) } @-}
-lem_csubst_conjunction :: CSub -> Expr -> Proof
-lem_csubst_conjunction (CEmpty)          p = ()
-lem_csubst_conjunction (CCons y v_y th)  p 
-  = () ? lem_csubst_conjunction th (subFV y v_y p ? lem_subFV_conjunction y v_y p)
-lem_csubst_conjunction (CConsT a t_a th) p 
-  = () ? lem_csubst_conjunction th (subFTV a t_a p ? lem_subFTV_conjunction a t_a p)
--}
-{-@ lem_csubst_strengthen :: th:CSub -> p:Pred -> q:Pred
-        -> { pf:_ | csubst th (strengthen p q) == strengthen (csubst th p) (csubst th q) } @-}
-lem_csubst_strengthen :: CSub -> Expr -> Expr -> Proof
-lem_csubst_strengthen (CEmpty)          p q = ()
-lem_csubst_strengthen (CCons  y v_y th) p q 
-  = () ? lem_subFV_strengthen y v_y p q
-       ? lem_csubst_strengthen th (subFV y v_y p) (subFV y v_y q)
-lem_csubst_strengthen (CConsT a t_a th) p q
-  = () ? lem_subFTV_strengthen a t_a p q
-       ? lem_csubst_strengthen th (subFTV a t_a p) (subFTV a t_a q)
-
-{-@ lem_ctsubst_push :: th:CSub -> p:Pred -> t_a:UserType
-        -> { pf:_ | ctsubst th (push p t_a) == push (csubst th p) (ctsubst th t_a) } @-}
-lem_ctsubst_push :: CSub -> Expr -> Type -> Proof
-lem_ctsubst_push (CEmpty)          p t_a = ()
-lem_ctsubst_push (CCons  y v_y th) p t_a 
-  = () ? lem_subFV_push y v_y p t_a
-       ? lem_ctsubst_push th (subFV y v_y p) (tsubFV y v_y t_a)
-lem_ctsubst_push (CConsT a' t' th) p t_a
-  = () ? lem_subFTV_push a' t' p t_a
-       ? lem_ctsubst_push th (subFTV a' t' p) (tsubFTV a' t' t_a)
-
-{-@ lem_ctsubst_erase_basic :: th:CSub -> t:Type 
-        -> { b:Basic | erase t == FTBasic b && (b == TBool || b == TInt) }
-        -> { pf:_ | erase (ctsubst th t) == FTBasic b } @-}
-lem_ctsubst_erase_basic :: CSub -> Type -> Basic -> Proof
-lem_ctsubst_erase_basic th (TRefn _b z p) b = case b of
-  TBool -> () ? lem_ctsubst_refn th TBool z p
-  TInt  -> () ? lem_ctsubst_refn th TInt  z p 
-lem_ctsubst_erase_basic th (TExists z t_z t) b 
-  = () ? lem_ctsubst_exis th z t_z t 
-       ? lem_ctsubst_erase_basic th t b
-
-{-@ lem_ctsubst_refn :: th:CSub -> { b:Basic | b == TBool || b == TInt || isBTV b } 
-               -> x:RVname -> p:Expr
-               -> { pf:_ | ctsubst th (TRefn b x p) == TRefn b x (csubst th p) } @-}
-lem_ctsubst_refn :: CSub -> Basic -> RVname -> Expr -> Proof
-lem_ctsubst_refn (CEmpty)       b x p    = ()
-lem_ctsubst_refn (CCons y v th) b x p    = () ? lem_ctsubst_refn th b x (subFV y v p)
-lem_ctsubst_refn (CConsT a t_a th) b x p = () ? lem_ctsubst_refn th b x (subFTV a t_a p)
-
-{-@ lem_ctsubst_refn_tv :: th:CSub -> { a:Vname | tv_in_csubst a th } -> x:RVname -> p:Pred
+Lemma lem_ctsubst_refn : forall (th:csub) (b:basic) (ps:preds),
+    isClosedBasic b \/ isBTV b 
+        -> ctsubst th (TRefn b ps) = TRefn b (cpsubst th ps).
+Proof. induction th; intros b ps Hb; simpl;
+  destruct b; simpl in Hb; try rewrite IHth; intuition. Qed.
+(* 33 *)
+(*
+{-@ lem_ctsubst_refn_tv :: th:csub -> { a:vname | tv_in_csubst a th } -> x:RVname -> p:preds
         -> { pf:_ | ctsubst th (TRefn (FTV a) x p) == push (csubst th p) (csubst_tv th a) } @-}
-lem_ctsubst_refn_tv :: CSub -> Vname -> RVname -> Expr -> Proof
+lem_ctsubst_refn_tv :: csub -> vname -> RVname -> expr -> Proof
 lem_ctsubst_refn_tv (CEmpty)          a x p = ()
 lem_ctsubst_refn_tv (CCons  y v_y th) a x p = () ? lem_ctsubst_refn_tv th a x (subFV y v_y p)
 lem_ctsubst_refn_tv (CConsT a' t' th) a x p 
@@ -295,17 +267,17 @@ lem_ctsubst_refn_tv (CConsT a' t' th) a x p
                    ? lem_ctsubst_nofree th t'
   | otherwise = () ? lem_ctsubst_refn_tv th a x (subFTV a' t' p)
 
-{-@ lem_ctsubst_refn_tv' :: th:CSub -> { a:Vname | tv_in_csubst a th } -> x:RVname -> p:Pred
+{-@ lem_ctsubst_refn_tv' :: th:csub -> { a:vname | tv_in_csubst a th } -> x:RVname -> p:preds
         -> { b:Basic | b == TBool || b == TInt } -> z:RVname
-        -> { q:Pred | (TRefn b z q) == csubst_tv th a }
+        -> { q:preds | (TRefn b z q) == csubst_tv th a }
         -> { pf:_ | ctsubst th (TRefn (FTV a) x p) == TRefn b z (strengthen (csubst th p) q) } @-}
-lem_ctsubst_refn_tv' :: CSub -> Vname -> RVname -> Expr -> Basic -> RVname -> Expr -> Proof
+lem_ctsubst_refn_tv' :: csub -> vname -> RVname -> expr -> Basic -> RVname -> expr -> Proof
 lem_ctsubst_refn_tv' th a x p b z q = () ? lem_ctsubst_refn_tv th a x p
 
-{-@ lem_ctsubst_refn_tv_notin :: th:CSub -> { a:Vname | not (tv_in_csubst a th) } 
-        -> x:RVname -> p:Expr 
+{-@ lem_ctsubst_refn_tv_notin :: th:csub -> { a:vname | not (tv_in_csubst a th) } 
+        -> x:RVname -> p:expr 
         -> { pf:_ | ctsubst th (TRefn (FTV a) x p) == TRefn (FTV a) x (csubst th p) } @-}
-lem_ctsubst_refn_tv_notin :: CSub -> Vname -> RVname -> Expr -> Proof
+lem_ctsubst_refn_tv_notin :: csub -> vname -> RVname -> expr -> Proof
 lem_ctsubst_refn_tv_notin (CEmpty)          a x p = ()
 lem_ctsubst_refn_tv_notin (CCons  y v_y th) a x p 
               = () ? lem_ctsubst_refn_tv_notin th a x (subFV y v_y p)
@@ -313,10 +285,10 @@ lem_ctsubst_refn_tv_notin (CConsT a' t' th) a x p
   | a == a'   = impossible ""
   | otherwise = () ? lem_ctsubst_refn_tv_notin th a x (subFTV a' t' p)
 
-{-@ lem_ctsubst_refn_usertype :: g:Env -> th:CSub -> ProofOf(DenotesEnv g th)
-        -> b:Basic -> x:RVname -> p:Pred -> ProofOf(WFType g (TRefn b x p) Base)
+{-@ lem_ctsubst_refn_usertype :: g:Env -> th:csub -> ProofOf(DenotesEnv g th)
+        -> b:Basic -> x:RVname -> p:preds -> ProofOf(WFType g (TRefn b x p) Base)
         -> { pf:_ | noExists (ctsubst th (TRefn b x p)) } @-}
-lem_ctsubst_refn_usertype :: Env -> CSub -> DenotesEnv -> Basic -> RVname -> Expr -> WFType -> Proof
+lem_ctsubst_refn_usertype :: Env -> csub -> DenotesEnv -> Basic -> RVname -> expr -> WFType -> Proof
 lem_ctsubst_refn_usertype g th den_g_th b x p p_g_t = case b of
   (FTV a) -> case ( csubst_tv th (a ? lem_wf_refn_tv_in_env g a x p Base p_g_t
                                     ? lem_binds_env_th g th den_g_th) ) of
@@ -328,36 +300,49 @@ lem_ctsubst_refn_usertype g th den_g_th b x p p_g_t = case b of
     (TPoly {})     -> () ? lem_ctsubst_refn_tv th a x p 
   _       -> () ? lem_ctsubst_refn    th b x p 
 
-{-@ lem_ctsubst_func :: th:CSub -> x:Vname -> t_x:Type -> t:Type
+{-@ lem_ctsubst_func :: th:csub -> x:vname -> t_x:type -> t:type
         -> { pf:_ | ctsubst th (TFunc x t_x t) == TFunc x (ctsubst th t_x) (ctsubst th t) } @-}  
-lem_ctsubst_func :: CSub -> Vname -> Type -> Type -> Proof
+lem_ctsubst_func :: csub -> vname -> type -> type -> Proof
 lem_ctsubst_func (CEmpty)       x t_x t = ()
 lem_ctsubst_func (CCons y v th) x t_x t 
     = () ? lem_ctsubst_func th x (tsubFV y v t_x) (tsubFV y v t) 
 lem_ctsubst_func (CConsT a t_a th) x t_x t 
     = () ? lem_ctsubst_func th x (tsubFTV a t_a t_x) (tsubFTV a t_a t)
 
-{-@ lem_ctsubst_exis :: th:CSub -> x:Vname -> t_x:Type -> t:Type
+{-@ lem_ctsubst_exis :: th:csub -> x:vname -> t_x:type -> t:type
         -> {pf:_ | ctsubst th (TExists x t_x t) == TExists x (ctsubst th t_x) (ctsubst th t)} @-}  
-lem_ctsubst_exis :: CSub -> Vname -> Type -> Type -> Proof
+lem_ctsubst_exis :: csub -> vname -> type -> type -> Proof
 lem_ctsubst_exis (CEmpty)       x t_x t = ()
 lem_ctsubst_exis (CCons y v th) x t_x t 
     = () ? lem_ctsubst_exis th x (tsubFV y v t_x) (tsubFV y v t) 
 lem_ctsubst_exis (CConsT a t_a th) x t_x t 
     = () ? lem_ctsubst_exis th x (tsubFTV a t_a t_x) (tsubFTV a t_a t)
 
-{-@ lem_ctsubst_poly :: th:CSub -> a:Vname -> k:Kind -> t:Type
+{-@ lem_ctsubst_poly :: th:csub -> a:vname -> k:kind -> t:type
         -> { pf:_ | ctsubst th (TPoly a k t) == TPoly a k (ctsubst th t) } @-}  
-lem_ctsubst_poly :: CSub -> Vname -> Kind -> Type -> Proof
+lem_ctsubst_poly :: csub -> vname -> kind -> type -> Proof
 lem_ctsubst_poly (CEmpty)           a k t = ()
 lem_ctsubst_poly (CCons  y  v   th) a k t  
     = () ? lem_ctsubst_poly th a k (tsubFV y v t) 
 lem_ctsubst_poly (CConsT a' t'  th) a k t 
     = () ? lem_ctsubst_poly th a k (tsubFTV a' t' t)
 
-{-@ lem_ctsubst_self :: th:CSub -> t:Type -> e:Term -> k:Kind 
+Lemma lem_ctsubst_erase_basic : forall (th:csub) (t:type) (b:basic), 
+    erase t = FTBasic b -> isClosedBasic b \/ isBTV b 
+        -> erase (ctsubst th t) = FTBasic b.
+Proof. intro th; induction t; simpl; intros; try discriminate;
+  rewrite <- H; rewrite lem_ctsubst_refn || rewrite lem_ctsubst_exis.
+lem_ctsubst_erase_basic th (TRefn _b z p) b = case b of
+  TBool -> () ? lem_ctsubst_refn th TBool z p
+  TInt  -> () ? lem_ctsubst_refn th TInt  z p 
+lem_ctsubst_erase_basic th (TExists z t_z t) b 
+  = () ? lem_ctsubst_exis th z t_z t 
+       ? lem_ctsubst_erase_basic th t b
+
+    
+{-@ lem_ctsubst_self :: th:csub -> t:type -> e:Term -> k:kind 
       -> { pf:_ | ctsubst th (self t e k) == self (ctsubst th t) (csubst th e) k } / [csubstSize th] @-}
-lem_ctsubst_self :: CSub -> Type -> Expr -> Kind -> Proof
+lem_ctsubst_self :: csub -> type -> expr -> kind -> Proof
 lem_ctsubst_self (CEmpty)          t e k = ()
 lem_ctsubst_self (CCons  y v_y th) t e k
   = () ? lem_tsubFV_self  y v_y t e k 
@@ -368,69 +353,60 @@ lem_ctsubst_self (CConsT a t_a th) t e k
 
   --- Various properties of csubst/ctsubst and free/bound variables
 
-{-@ lem_csubst_binds :: g:Env -> th:CSub -> ProofOf(DenotesEnv g th) 
-        -> { pf:_ | binds g == bindsC th && vbinds g == vbindsC th && tvbinds g == tvbindsC th} @-}
-lem_csubst_binds :: Env -> CSub -> DenotesEnv -> Proof
-lem_csubst_binds g th DEmp                                             = ()
-lem_csubst_binds g th (DExt  g' th' den_g'_th' x t_x v_x den_th'tx_vx) 
-    = () ? lem_csubst_binds g' th' den_g'_th'
-lem_csubst_binds g th (DExtT g' th' den_g'_th' a k_a t_a p_emp_ta)
-    = () ? lem_csubst_binds g' th' den_g'_th'
-
-{-@ lem_csubst_nofv :: th:CSub -> { e:Expr | Set_emp (fv e) && Set_emp (ftv e) }
+{-@ lem_csubst_nofv :: th:csub -> { e:expr | Set_emp (fv e) && Set_emp (ftv e) }
         -> { pf:_ | csubst th e == e } @-}
-lem_csubst_nofv :: CSub -> Expr -> Proof
+lem_csubst_nofv :: csub -> expr -> Proof
 lem_csubst_nofv (CEmpty)       e    = ()
 lem_csubst_nofv (CCons x v th) e    = () ? lem_csubst_nofv th e
                                          ? lem_subFV_notin x v e
 lem_csubst_nofv (CConsT a t_a th) e = () ? lem_csubst_nofv th e
                                          ? lem_subFTV_notin a t_a e 
 
-{-@ lem_ctsubst_nofree :: th:CSub -> { t:Type | Set_emp (free t) && Set_emp (freeTV t) }
+{-@ lem_ctsubst_nofree :: th:csub -> { t:type | Set_emp (free t) && Set_emp (freeTV t) }
         -> { pf:_ | ctsubst th t == t } @-}
-lem_ctsubst_nofree :: CSub -> Type -> Proof
+lem_ctsubst_nofree :: csub -> type -> Proof
 lem_ctsubst_nofree (CEmpty)          t = ()
 lem_ctsubst_nofree (CCons x v th)    t = () ? lem_ctsubst_nofree th t
                                             ? lem_tsubFV_notin x v t 
 lem_ctsubst_nofree (CConsT a t_a th) t = () ? lem_ctsubst_nofree th t
                                             ? lem_tsubFTV_notin a t_a t 
 
-{-{-@ lem_csubst_freeBV :: th:CSub -> e:Expr
+{-{-@ lem_csubst_freeBV :: th:csub -> e:expr
         -> { pf:_ | freeBV (csubst th e) == freeBV e } @-}
-lem_csubst_freeBV :: CSub -> Expr -> Proof
+lem_csubst_freeBV :: csub -> expr -> Proof
 lem_csubst_freeBV (CEmpty)       e = ()
 lem_csubst_freeBV (CCons x v th) e = () ? lem_csubst_freeBV th (subFV x v e)
                          ? toProof ( freeBV (subFV x v e) === freeBV e )
 -}
-{-@ lem_ctsubst_nofreeBV :: th:CSub -> { t:Type | Set_emp (tfreeBV t) }
+{-@ lem_ctsubst_nofreeBV :: th:csub -> { t:type | Set_emp (tfreeBV t) }
         -> { pf:_ | Set_emp (tfreeBV (ctsubst th t)) } @-}
-lem_ctsubst_nofreeBV :: CSub -> Type -> Proof
+lem_ctsubst_nofreeBV :: csub -> type -> Proof
 lem_ctsubst_nofreeBV (CEmpty)          t = ()
 lem_ctsubst_nofreeBV (CCons x v th)    t = () ? lem_ctsubst_nofreeBV th (tsubFV x v t
                                                     ? lem_tsubFV_tfreeBV  x v   t)
 lem_ctsubst_nofreeBV (CConsT a t_a th) t = () ? lem_ctsubst_nofreeBV th (tsubFTV a t_a t
                                                     ? lem_tsubFTV_tfreeBV a t_a t)
 
-{-@ lem_csubst_value :: th:CSub -> v:Value  
+{-@ lem_csubst_value :: th:csub -> v:Value  
         -> { pf:_ | isValue (csubst th v) && isTerm (csubst th v) } @-}
-lem_csubst_value :: CSub -> Expr -> Proof
+lem_csubst_value :: csub -> expr -> Proof
 lem_csubst_value (CEmpty)          v = ()
 lem_csubst_value (CCons y v_y th)  v = () ? lem_csubst_value th (subFV y v_y v)
 lem_csubst_value (CConsT a t_a th) v = () ? lem_csubst_value th (subFTV a t_a v)
 
-{-@ lem_ctsubst_usertype :: th:CSub -> t_a:UserType -> { pf:_ | noExists (ctsubst th t_a) } @-}
-lem_ctsubst_usertype :: CSub -> Type -> Proof
+{-@ lem_ctsubst_usertype :: th:csub -> t_a:UserType -> { pf:_ | noExists (ctsubst th t_a) } @-}
+lem_ctsubst_usertype :: csub -> type -> Proof
 lem_ctsubst_usertype (CEmpty)          t = ()
 lem_ctsubst_usertype (CCons y v_y th)  t = () ? lem_ctsubst_usertype th (tsubFV y v_y t)
 lem_ctsubst_usertype (CConsT a t_a th) t = () ? lem_ctsubst_usertype th (tsubFTV a t_a t)
 
-{-@ lem_ctsubst_head_not_free :: x:Vname 
+{-@ lem_ctsubst_head_not_free :: x:vname 
         -> { v_x:Value | Set_emp (fv v_x) && Set_emp (ftv v_x) &&
                          Set_emp (freeBV v_x) && Set_emp (freeBTV v_x) } 
-        -> { th:CSub | not (Set_mem x (bindsC th)) }
-        -> { t:Type | not (Set_mem x (free t)) } 
+        -> { th:csub | not (Set_mem x (bindsC th)) }
+        -> { t:type | not (Set_mem x (free t)) } 
         -> { pf:_ | ctsubst (CCons x v_x th) t == ctsubst th t } @-}
-lem_ctsubst_head_not_free :: Vname -> Expr -> CSub -> Type -> Proof
+lem_ctsubst_head_not_free :: vname -> expr -> csub -> type -> Proof
 lem_ctsubst_head_not_free x v_x th t = toProof ( ctsubst (CCons x v_x th) t
                                              === ctsubst th (tsubFV x v_x t)
                                              === ctsubst th t )
@@ -438,10 +414,10 @@ lem_ctsubst_head_not_free x v_x th t = toProof ( ctsubst (CCons x v_x th) t
   --- Commutative laws relating csubst/ctsubst and substitution operations
   --- The first set of these laws involve [v/x] or [t_a/a] where v or t_a have no free vars
 
-{-@ lem_csubst_subBV :: x:Vname -> v:Value -> bt:FType 
-           -> ProofOf(HasFType FEmpty v bt) -> th:CSub -> p:Expr
+{-@ lem_csubst_subBV :: x:vname -> v:Value -> bt:FType 
+           -> ProofOf(HasFType FEmpty v bt) -> th:csub -> p:expr
            -> { pf:_ | csubst th (subBV x v p) == subBV x v (csubst th p) } @-}
-lem_csubst_subBV :: Vname -> Expr -> FType -> HasFType -> CSub -> Expr -> Proof
+lem_csubst_subBV :: vname -> expr -> FType -> HasFType -> csub -> expr -> Proof
 lem_csubst_subBV x v bt pf_v_b (CEmpty)         p = ()
 lem_csubst_subBV x v bt pf_v_b (CCons y v_y th) p 
     = () ? lem_commute_subFV_subBV1 x v 
@@ -452,10 +428,10 @@ lem_csubst_subBV x v bt pf_v_b (CConsT a t_a th) p
                    (a `withProof` lem_fv_bound_in_fenv FEmpty v bt pf_v_b a) t_a p
          ? lem_csubst_subBV x v bt pf_v_b th (subFTV a t_a p)
 
-{-@ lem_csubst_subBTV :: a:Vname -> t_a:UserType -> k:Kind 
-           -> ProofOf(WFType Empty t_a k) -> th:CSub -> p:Expr
+{-@ lem_csubst_subBTV :: a:vname -> t_a:UserType -> k:kind 
+           -> ProofOf(WFType Empty t_a k) -> th:csub -> p:expr
            -> { pf:_ | csubst th (subBTV a t_a p) == subBTV a t_a (csubst th p) } @-}
-lem_csubst_subBTV :: Vname -> Type -> Kind -> WFType -> CSub -> Expr -> Proof
+lem_csubst_subBTV :: vname -> type -> kind -> WFType -> csub -> expr -> Proof
 lem_csubst_subBTV a t_a k p_emp_ta (CEmpty)          p = ()
 lem_csubst_subBTV a t_a k p_emp_ta (CCons y v_y th)  p 
   = () ? lem_commute_subFV_subBTV1 a t_a 
@@ -466,10 +442,10 @@ lem_csubst_subBTV a t_a k p_emp_ta (CConsT a1 t1 th) p
              (a1 ? lem_free_bound_in_env Empty t_a k p_emp_ta a1) t1 p
        ? lem_csubst_subBTV a t_a k p_emp_ta th (subFTV a1 t1 p)
 
-{-@ lem_ctsubst_tsubBV :: x:Vname -> v:Value -> bt:FType
-           -> ProofOf(HasFType FEmpty v bt) -> th:CSub -> t:Type
+{-@ lem_ctsubst_tsubBV :: x:vname -> v:Value -> bt:FType
+           -> ProofOf(HasFType FEmpty v bt) -> th:csub -> t:type
            -> { pf:_ | ctsubst th (tsubBV x v t) == tsubBV x v (ctsubst th t) } @-}
-lem_ctsubst_tsubBV :: Vname -> Expr -> FType -> HasFType -> CSub -> Type -> Proof
+lem_ctsubst_tsubBV :: vname -> expr -> FType -> HasFType -> csub -> type -> Proof
 lem_ctsubst_tsubBV x v bt pf_v_b (CEmpty)         t = ()
 lem_ctsubst_tsubBV x v bt pf_v_b (CCons y v_y th) t 
     = () ? lem_commute_tsubFV_tsubBV1 x v 
@@ -480,10 +456,10 @@ lem_ctsubst_tsubBV x v bt pf_v_b (CConsT a t_a th) t
                    (a `withProof` lem_fv_bound_in_fenv FEmpty v bt pf_v_b a) t_a t
          ? lem_ctsubst_tsubBV x v bt pf_v_b th (tsubFTV a t_a t)
 
-{-@ lem_ctsubst_tsubBTV :: a1:Vname -> t_a:UserType -> k:Kind 
-        -> ProofOf(WFType Empty t_a k) -> th:CSub -> t:Type 
+{-@ lem_ctsubst_tsubBTV :: a1:vname -> t_a:UserType -> k:kind 
+        -> ProofOf(WFType Empty t_a k) -> th:csub -> t:type 
         -> { pf:_ | ctsubst th (tsubBTV a1 t_a t) == tsubBTV a1 t_a (ctsubst th t) } @-}
-lem_ctsubst_tsubBTV :: Vname -> Type -> Kind -> WFType -> CSub -> Type -> Proof
+lem_ctsubst_tsubBTV :: vname -> type -> kind -> WFType -> csub -> type -> Proof
 lem_ctsubst_tsubBTV a1 t_a k p_emp_ta (CEmpty)            t = ()
 lem_ctsubst_tsubBTV a1 t_a k p_emp_ta (CCons y v_y th)    t
     = () ? lem_commute_tsubFV_tsubBTV1 a1 t_a
@@ -496,9 +472,9 @@ lem_ctsubst_tsubBTV a1 t_a k p_emp_ta (CConsT a' t_a' th) t
 
   --- The second set of these laws are more general for [v/x] or [t_a/a] incl free vars
 
-{-@ lem_commute_csubst_subBV :: th:CSub -> x:Vname -> v:Value -> e:Expr
+{-@ lem_commute_csubst_subBV :: th:csub -> x:vname -> v:Value -> e:expr
            -> { pf:_ | csubst th (subBV x v e) == subBV x (csubst th v) (csubst th e) } @-} 
-lem_commute_csubst_subBV :: CSub -> Vname -> Expr -> Expr -> Proof
+lem_commute_csubst_subBV :: csub -> vname -> expr -> expr -> Proof
 lem_commute_csubst_subBV (CEmpty)         x v e = () 
 lem_commute_csubst_subBV (CCons y v_y th) x v e 
     = () ? lem_commute_subFV_subBV x v y v_y e
@@ -507,9 +483,9 @@ lem_commute_csubst_subBV (CConsT a t_a th) x v e
     = () ? lem_commute_subFTV_subBV x v a t_a e
          ? lem_commute_csubst_subBV th x (subFTV a t_a v) (subFTV a t_a e)
 
-{-@ lem_commute_csubst_subBTV :: th:CSub -> a:Vname -> t_a:UserType -> e:Expr
+{-@ lem_commute_csubst_subBTV :: th:csub -> a:vname -> t_a:UserType -> e:expr
             -> { pf:_ | csubst th (subBTV a t_a e) == subBTV a (ctsubst th t_a) (csubst th e) } @-}
-lem_commute_csubst_subBTV :: CSub -> Vname -> Type -> Expr -> Proof
+lem_commute_csubst_subBTV :: csub -> vname -> type -> expr -> Proof
 lem_commute_csubst_subBTV (CEmpty)          a t_a e = ()
 lem_commute_csubst_subBTV (CCons  y v_y th) a t_a e
     = () ? lem_commute_subFV_subBTV a t_a y v_y e
@@ -518,9 +494,9 @@ lem_commute_csubst_subBTV (CConsT a' t' th) a t_a e
     = () ? lem_commute_subFTV_subBTV a t_a a' t' e
          ? lem_commute_csubst_subBTV th a (tsubFTV a' t' t_a) (subFTV a' t' e)
 
-{-@ lem_commute_ctsubst_tsubBV :: th:CSub -> x:Vname -> v:Value -> t:Type
+{-@ lem_commute_ctsubst_tsubBV :: th:csub -> x:vname -> v:Value -> t:type
            -> { pf:_ | ctsubst th (tsubBV x v t) == tsubBV x (csubst th v) (ctsubst th t) } @-} 
-lem_commute_ctsubst_tsubBV :: CSub -> Vname -> Expr -> Type -> Proof
+lem_commute_ctsubst_tsubBV :: csub -> vname -> expr -> type -> Proof
 lem_commute_ctsubst_tsubBV (CEmpty)         x v t = () 
 lem_commute_ctsubst_tsubBV (CCons y v_y th) x v t 
     = () ? lem_commute_tsubFV_tsubBV x v y v_y t
@@ -529,9 +505,9 @@ lem_commute_ctsubst_tsubBV (CConsT a t_a th) x v t
     = () ? lem_commute_tsubFTV_tsubBV x v a t_a t
          ? lem_commute_ctsubst_tsubBV th x (subFTV a t_a v) (tsubFTV a t_a t)
 
-{-@ lem_commute_ctsubst_tsubBTV :: th:CSub -> a:Vname -> t_a:UserType -> t:Type 
+{-@ lem_commute_ctsubst_tsubBTV :: th:csub -> a:vname -> t_a:UserType -> t:type 
         -> { pf:_ | ctsubst th (tsubBTV a t_a t) == tsubBTV a (ctsubst th t_a) (ctsubst th t) } @-}
-lem_commute_ctsubst_tsubBTV :: CSub -> Vname -> Type -> Type -> Proof
+lem_commute_ctsubst_tsubBTV :: csub -> vname -> type -> type -> Proof
 lem_commute_ctsubst_tsubBTV (CEmpty)            a t_a t = ()
 lem_commute_ctsubst_tsubBTV (CCons y v_y th)    a t_a t  
     = () ? lem_commute_tsubFV_tsubBTV a t_a y v_y t
@@ -543,11 +519,11 @@ lem_commute_ctsubst_tsubBTV (CConsT a' t_a' th) a t_a t
 
   --- Compositional Laws
 
-{-@ lem_csubst_and_unbind :: x:Vname -> y:Vname 
+{-@ lem_csubst_and_unbind :: x:vname -> y:vname 
            -> v:Value -> bt:FType -> ProofOf(HasFType FEmpty v bt)
-           -> { th:CSub | not (Set_mem y (bindsC th)) } -> { p:Expr | not (Set_mem y (fv p)) }
+           -> { th:csub | not (Set_mem y (bindsC th)) } -> { p:expr | not (Set_mem y (fv p)) }
            -> { pf:_ | csubst (CCons y v th) (unbind x y p) == subBV x v (csubst th p) } @-}
-lem_csubst_and_unbind :: Vname -> Vname -> Expr -> FType -> HasFType -> CSub -> Expr -> Proof
+lem_csubst_and_unbind :: vname -> vname -> expr -> FType -> HasFType -> csub -> expr -> Proof
 lem_csubst_and_unbind x y v b pf_v_b th p = () {-toProof ( 
        csubst (CCons y (v-}  ? lem_fv_subset_bindsF FEmpty v b pf_v_b{-) th) (unbind x y p) 
    === csubst th (subFV y v (unbind x y p))-}
@@ -556,22 +532,22 @@ lem_csubst_and_unbind x y v b pf_v_b th p = () {-toProof (
      ? lem_csubst_subBV x v b pf_v_b th p
 --   === subBV x v (csubst th p) )
 
-{-@ lem_csubst_and_unbind_tv :: a:Vname -> a':Vname -> t_a:UserType -> k:Kind -> ProofOf(WFType Empty t_a k)
-        -> { th:CSub | not (Set_mem a' (bindsC th)) } -> { p:Expr | not (Set_mem a' (ftv p)) }
+{-@ lem_csubst_and_unbind_tv :: a:vname -> a':vname -> t_a:UserType -> k:kind -> ProofOf(WFType Empty t_a k)
+        -> { th:csub | not (Set_mem a' (bindsC th)) } -> { p:expr | not (Set_mem a' (ftv p)) }
         -> { pf:_ | csubst (CConsT a' t_a th) (unbind_tv a a' p) == subBTV a t_a (csubst th p) } @-}
-lem_csubst_and_unbind_tv :: Vname -> Vname -> Type -> Kind -> WFType -> CSub -> Expr -> Proof
+lem_csubst_and_unbind_tv :: vname -> vname -> type -> kind -> WFType -> csub -> expr -> Proof
 lem_csubst_and_unbind_tv a a' t_a k pf_emp_ta th p 
   = () ? lem_free_subset_binds Empty t_a k pf_emp_ta  
        ? lem_tfreeBV_empty     Empty t_a k pf_emp_ta 
        ? lem_subFTV_unbind_tv  a a' t_a p
        ? lem_csubst_subBTV     a t_a k pf_emp_ta th p
 
-{-@ lem_ctsubst_and_unbindT :: x:Vname -> y:Vname
+{-@ lem_ctsubst_and_unbindT :: x:vname -> y:vname
            -> v:Value -> bt:FType -> ProofOf(HasFType FEmpty v bt)
-           -> { th:CSub | not (Set_mem y (bindsC th)) } -> { t:Type | not (Set_mem y (free t)) }
+           -> { th:csub | not (Set_mem y (bindsC th)) } -> { t:type | not (Set_mem y (free t)) }
            -> { pf:_ | ctsubst (CCons y v th) (unbindT x y t) == tsubBV x v (ctsubst th t) } @-}
-lem_ctsubst_and_unbindT :: Vname -> Vname -> Expr -> FType -> HasFType 
-           -> CSub -> Type -> Proof
+lem_ctsubst_and_unbindT :: vname -> vname -> expr -> FType -> HasFType 
+           -> csub -> type -> Proof
 lem_ctsubst_and_unbindT x y v bt pf_v_b th t = () {-toProof ( 
        ctsubst (CCons y (v-} ? lem_fv_subset_bindsF FEmpty v bt pf_v_b{-) th) (unbindT x y t)
    === ctsubst th (tsubFV y v (unbindT x y t))-}
@@ -580,12 +556,12 @@ lem_ctsubst_and_unbindT x y v bt pf_v_b th t = () {-toProof (
      ? lem_ctsubst_tsubBV x v bt pf_v_b th t
 --   === tsubBV x v (ctsubst th t) )
 
-{-@ lem_ctsubst_and_unbind_tvT :: a1:Vname -> a:Vname -> t_a:UserType 
-        -> k:Kind -> ProofOf(WFType Empty t_a k)
-        -> { th:CSub | not (Set_mem a (bindsC th)) } -> { t:Type | not (Set_mem a (freeTV t)) }
+{-@ lem_ctsubst_and_unbind_tvT :: a1:vname -> a:vname -> t_a:UserType 
+        -> k:kind -> ProofOf(WFType Empty t_a k)
+        -> { th:csub | not (Set_mem a (bindsC th)) } -> { t:type | not (Set_mem a (freeTV t)) }
         -> { pf:_ | ctsubst (CConsT a t_a th) (unbind_tvT a1 a t) == tsubBTV a1 t_a (ctsubst th t) } @-}
-lem_ctsubst_and_unbind_tvT :: Vname -> Vname -> Type -> Kind -> WFType  
-           -> CSub -> Type -> Proof
+lem_ctsubst_and_unbind_tvT :: vname -> vname -> type -> kind -> WFType  
+           -> csub -> type -> Proof
 lem_ctsubst_and_unbind_tvT a1 a t_a k p_emp_ta th t 
   = () ? lem_free_subset_binds  Empty t_a k p_emp_ta
        ? lem_tfreeBV_empty      Empty t_a k p_emp_ta 
@@ -594,41 +570,41 @@ lem_ctsubst_and_unbind_tvT a1 a t_a k p_emp_ta th t
 
   --- After applying a closing substitution there are no more free variables remaining
 
-{-@ lem_csubst_no_more_fv :: th:CSub 
-        -> { v_x:Expr | Set_sub (fv v_x) (vbindsC th) && Set_sub (ftv v_x) (tvbindsC th) }
+{-@ lem_csubst_no_more_fv :: th:csub 
+        -> { v_x:expr | Set_sub (fv v_x) (vbindsC th) && Set_sub (ftv v_x) (tvbindsC th) }
         -> { pf:_ | Set_emp (fv (csubst th v_x)) && Set_emp (ftv (csubst th v_x)) } @-}
-lem_csubst_no_more_fv :: CSub -> Expr -> Proof
+lem_csubst_no_more_fv :: csub -> expr -> Proof
 lem_csubst_no_more_fv CEmpty v_x            = ()
 lem_csubst_no_more_fv (CCons  y v_y th) v_x = () ? lem_csubst_no_more_fv th (subFV y v_y v_x)
 lem_csubst_no_more_fv (CConsT a t_a th) v_x = () ? lem_csubst_no_more_fv th (subFTV a t_a v_x)
 
-{-@ lem_ctsubst_no_more_fv :: th:CSub 
-        -> { t:Type | Set_sub (free t) (vbindsC th) && Set_sub (freeTV t) (tvbindsC th) }
+{-@ lem_ctsubst_no_more_fv :: th:csub 
+        -> { t:type | Set_sub (free t) (vbindsC th) && Set_sub (freeTV t) (tvbindsC th) }
         -> { pf:_ | Set_emp (free (ctsubst th t)) && Set_emp (freeTV (ctsubst th t)) } @-}
-lem_ctsubst_no_more_fv :: CSub -> Type -> Proof
+lem_ctsubst_no_more_fv :: csub -> type -> Proof
 lem_ctsubst_no_more_fv CEmpty            t = ()
 lem_ctsubst_no_more_fv (CCons  y v_y th) t = () ? lem_ctsubst_no_more_fv th (tsubFV y v_y t)
 lem_ctsubst_no_more_fv (CConsT a t_a th) t = () ? lem_ctsubst_no_more_fv th (tsubFTV a t_a t)
     
-{-@ lem_csubst_no_more_bv :: th:CSub 
-        -> { v_x:Expr | Set_emp (freeBV v_x) && Set_emp (freeBTV v_x) }
+{-@ lem_csubst_no_more_bv :: th:csub 
+        -> { v_x:expr | Set_emp (freeBV v_x) && Set_emp (freeBTV v_x) }
         -> { pf:_ | Set_emp (freeBV (csubst th v_x)) && Set_emp (freeBTV (csubst th v_x)) } @-}
-lem_csubst_no_more_bv :: CSub -> Expr -> Proof
+lem_csubst_no_more_bv :: csub -> expr -> Proof
 lem_csubst_no_more_bv CEmpty v_x            = ()
 lem_csubst_no_more_bv (CCons  y v_y th) v_x = () ? lem_csubst_no_more_bv th (subFV y v_y v_x)
 lem_csubst_no_more_bv (CConsT a t_a th) v_x = () ? lem_csubst_no_more_bv th (subFTV a t_a v_x)
 
-{-@ lem_ctsubst_no_more_bv :: th:CSub -> { t:Type | Set_emp (tfreeBV t) && Set_emp (tfreeBTV t) }
+{-@ lem_ctsubst_no_more_bv :: th:csub -> { t:type | Set_emp (tfreeBV t) && Set_emp (tfreeBTV t) }
         -> { pf:_ | Set_emp (tfreeBV (ctsubst th t)) && Set_emp (tfreeBTV (ctsubst th t)) } @-}
-lem_ctsubst_no_more_bv :: CSub -> Type -> Proof
+lem_ctsubst_no_more_bv :: csub -> type -> Proof
 lem_ctsubst_no_more_bv CEmpty            t = ()
 lem_ctsubst_no_more_bv (CCons  y v_y th) t = () ? lem_ctsubst_no_more_bv th (tsubFV y v_y t)
 lem_ctsubst_no_more_bv (CConsT a t_a th) t = () ? lem_ctsubst_no_more_bv th (tsubFTV a t_a t)
 
-{-@ lem_csubst_subFV :: th:CSub -> { x:Vname | not (in_csubst x th) } 
-        -> { v_x:Value | Set_sub (fv v_x) (vbindsC th) && Set_sub (ftv v_x) (tvbindsC th) } -> e:Expr
+{-@ lem_csubst_subFV :: th:csub -> { x:vname | not (in_csubst x th) } 
+        -> { v_x:Value | Set_sub (fv v_x) (vbindsC th) && Set_sub (ftv v_x) (tvbindsC th) } -> e:expr
         -> { pf:_ | csubst th (subFV x v_x e) == csubst th (subFV x (csubst th v_x) e) } @-}
-lem_csubst_subFV :: CSub -> Vname -> Expr -> Expr -> Proof
+lem_csubst_subFV :: csub -> vname -> expr -> expr -> Proof
 lem_csubst_subFV  CEmpty            x v_x e = ()
 lem_csubst_subFV  (CCons y v_y th)  x v_x e 
   = () -- ? toProof (
@@ -654,10 +630,10 @@ lem_csubst_subFV  (CConsT a t_a th) x v_x e
          ? lem_csubst_subFV th x (subFTV a t_a v_x) (subFTV a t_a e)
          ? lem_commute_subFTV_subFV x v_x a t_a e
     
-{-@ lem_ctsubst_tsubFV :: th:CSub -> { x:Vname | not (in_csubst x th) } 
-        -> { v_x:Value | Set_sub (fv v_x) (vbindsC th) && Set_sub (ftv v_x) (tvbindsC th) } -> t:Type
+{-@ lem_ctsubst_tsubFV :: th:csub -> { x:vname | not (in_csubst x th) } 
+        -> { v_x:Value | Set_sub (fv v_x) (vbindsC th) && Set_sub (ftv v_x) (tvbindsC th) } -> t:type
         -> { pf:_ | ctsubst th (tsubFV x v_x t) == ctsubst th (tsubFV x (csubst th v_x) t) } @-}
-lem_ctsubst_tsubFV :: CSub -> Vname -> Expr -> Type -> Proof
+lem_ctsubst_tsubFV :: csub -> vname -> expr -> type -> Proof
 lem_ctsubst_tsubFV  CEmpty            x v_x t = ()
 lem_ctsubst_tsubFV  (CCons y v_y th)  x v_x t 
   = () -- ? toProof (
@@ -684,10 +660,10 @@ lem_ctsubst_tsubFV  (CConsT a t_a th) x v_x t
          ? lem_ctsubst_tsubFV th x (subFTV a t_a v_x) (tsubFTV a t_a t)
          ? lem_commute_tsubFTV_tsubFV x v_x a t_a t
 
-{-@ lem_csubst_subFTV :: th:CSub -> { a:Vname | not (in_csubst a th) } 
+{-@ lem_csubst_subFTV :: th:csub -> { a:vname | not (in_csubst a th) } 
         -> { t_a:UserType | Set_sub (free t_a) (vbindsC th) && Set_sub (freeTV t_a) (tvbindsC th) } 
-        -> e:Expr -> { pf:_ | csubst th (subFTV a t_a e) == csubst th (subFTV a (ctsubst th t_a) e) } @-}
-lem_csubst_subFTV :: CSub -> Vname -> Type -> Expr -> Proof
+        -> e:expr -> { pf:_ | csubst th (subFTV a t_a e) == csubst th (subFTV a (ctsubst th t_a) e) } @-}
+lem_csubst_subFTV :: csub -> vname -> type -> expr -> Proof
 lem_csubst_subFTV  CEmpty            a t_a e = ()
 lem_csubst_subFTV  (CCons y v_y th)  a t_a e 
   = ()  ? lem_commute_subFV_subFTV a (ctsubst (CCons y v_y th) t_a 
@@ -704,10 +680,10 @@ lem_csubst_subFTV  (CConsT a' t_a' th) a t_a e
          ? lem_csubst_subFTV th a (tsubFTV a' t_a' t_a) (subFTV a' t_a' e)
          ? lem_commute_subFTV a t_a a' t_a' e
     
-{-@ lem_ctsubst_tsubFTV :: th:CSub -> { a:Vname | not (in_csubst a th) } 
+{-@ lem_ctsubst_tsubFTV :: th:csub -> { a:vname | not (in_csubst a th) } 
         -> { t_a:UserType | Set_sub (free t_a) (vbindsC th) && Set_sub (freeTV t_a) (tvbindsC th) } 
-        -> t:Type -> {pf:_ | ctsubst th (tsubFTV a t_a t) == ctsubst th (tsubFTV a (ctsubst th t_a) t)} @-}
-lem_ctsubst_tsubFTV :: CSub -> Vname -> Type -> Type -> Proof
+        -> t:type -> {pf:_ | ctsubst th (tsubFTV a t_a t) == ctsubst th (tsubFTV a (ctsubst th t_a) t)} @-}
+lem_ctsubst_tsubFTV :: csub -> vname -> type -> type -> Proof
 lem_ctsubst_tsubFTV  CEmpty            a t_a t = ()
 lem_ctsubst_tsubFTV  (CCons y v_y th)  a t_a t 
   = ()  ? lem_commute_tsubFV_tsubFTV a (ctsubst (CCons y v_y th) t_a 
@@ -726,12 +702,12 @@ lem_ctsubst_tsubFTV  (CConsT a' t_a' th) a t_a t
 
   --- Closing Substitutions and Technical Operations
 
-        -- -> { e:Expr | Set_sub (fv e) (bindsC th ) && ( x == y || not (Set_mem y (fv e))) }
-{-@ lem_change_var_in_csubst :: th:CSub -> { x:Vname | v_in_csubst x th }
-        -> { y:Vname  | y == x || not (in_csubst y th) }
-        -> { e:Expr   | x == y || not (Set_mem y (fv e)) }
+        -- -> { e:expr | Set_sub (fv e) (bindsC th ) && ( x == y || not (Set_mem y (fv e))) }
+{-@ lem_change_var_in_csubst :: th:csub -> { x:vname | v_in_csubst x th }
+        -> { y:vname  | y == x || not (in_csubst y th) }
+        -> { e:expr   | x == y || not (Set_mem y (fv e)) }
         -> { pf:Proof | csubst th e == csubst (change_varCS th x y) (subFV x (FV y) e) } @-}
-lem_change_var_in_csubst :: CSub -> Vname -> Vname -> Expr -> Proof
+lem_change_var_in_csubst :: csub -> vname -> vname -> expr -> Proof
 lem_change_var_in_csubst (CCons z v_z th) x y e = case (x == z) of
   (True)  -> () {- toProof ( csubst (change_varCS (CCons z v_z th) x y) (subFV x (FV y) e)
                    === csubst (CCons y v_z th) (subFV x (FV y) e)
@@ -755,11 +731,11 @@ lem_change_var_in_csubst (CConsT a t_a th) x y e
          ? lem_tsubFV_notin x (FV y) t_a
          ? lem_change_var_in_csubst th x y (subFTV a t_a e)
 
-{-@ lem_change_tvar_in_csubst :: th:CSub -> { a:Vname | tv_in_csubst a th }
-        -> { a':Vname | a == a' || not (in_csubst a' th) }
-        -> { e:Expr   | a == a' || not (Set_mem a' (ftv e)) }
+{-@ lem_change_tvar_in_csubst :: th:csub -> { a:vname | tv_in_csubst a th }
+        -> { a':vname | a == a' || not (in_csubst a' th) }
+        -> { e:expr   | a == a' || not (Set_mem a' (ftv e)) }
         -> { pf:Proof | csubst th e == csubst (change_tvarCS th a a') (chgFTV a a' e) } @-}
-lem_change_tvar_in_csubst :: CSub -> Vname -> Vname -> Expr -> Proof
+lem_change_tvar_in_csubst :: csub -> vname -> vname -> expr -> Proof
 lem_change_tvar_in_csubst (CCons   z v_z th) a a' e 
   = () ? lem_commute_chgFTV_subFV  z v_z a a' e
        ? lem_chgFTV_notin a a' v_z
@@ -770,12 +746,12 @@ lem_change_tvar_in_csubst (CConsT a1 t_a th) a a' e = case ( a == a1 ) of
                 ? lem_tchgFTV_notin a a' t_a
                 ? lem_change_tvar_in_csubst th a a' (subFTV a1 t_a e)
 
-        -- -> { t:Type | Set_sub (free t) (bindsC th ) && ( x == y || not (Set_mem y (free t))) }
-{-@ lem_change_var_in_ctsubst :: th:CSub -> { x:Vname | v_in_csubst x th }
-        -> { y:Vname  | y == x || not (in_csubst y th) }
-        -> { t:Type   | x == y || not (Set_mem y (free t)) }
+        -- -> { t:type | Set_sub (free t) (bindsC th ) && ( x == y || not (Set_mem y (free t))) }
+{-@ lem_change_var_in_ctsubst :: th:csub -> { x:vname | v_in_csubst x th }
+        -> { y:vname  | y == x || not (in_csubst y th) }
+        -> { t:type   | x == y || not (Set_mem y (free t)) }
         -> { pf:Proof | ctsubst th t == ctsubst (change_varCS th x y) (tsubFV x (FV y) t) } @-}
-lem_change_var_in_ctsubst :: CSub -> Vname -> Vname -> Type -> Proof
+lem_change_var_in_ctsubst :: csub -> vname -> vname -> type -> Proof
 lem_change_var_in_ctsubst (CCons z v_z th) x y t = case (x == z) of
   (True)  -> () ? lem_chain_tsubFV x y v_z t 
   (False) -> () ? lem_commute_tsubFV x (FV y) z v_z t
@@ -785,11 +761,11 @@ lem_change_var_in_ctsubst (CConsT a t_a th) x y t
          ? lem_tsubFV_notin x (FV y) t_a
          ? lem_change_var_in_ctsubst th x y (tsubFTV a t_a t)
 
-{-@ lem_change_tvar_in_ctsubst :: th:CSub -> { a:Vname | tv_in_csubst a th }
-        -> { a':Vname | a == a' || not (in_csubst a' th) }
-        -> { t:Type   | a == a' || not (Set_mem a' (freeTV t)) }
+{-@ lem_change_tvar_in_ctsubst :: th:csub -> { a:vname | tv_in_csubst a th }
+        -> { a':vname | a == a' || not (in_csubst a' th) }
+        -> { t:type   | a == a' || not (Set_mem a' (freeTV t)) }
         -> { pf:Proof | ctsubst th t == ctsubst (change_tvarCS th a a') (tchgFTV a a' t) } @-}
-lem_change_tvar_in_ctsubst :: CSub -> Vname -> Vname -> Type -> Proof
+lem_change_tvar_in_ctsubst :: csub -> vname -> vname -> type -> Proof
 lem_change_tvar_in_ctsubst (CCons z v_z th) a a' t 
   = () ? lem_commute_tchgFTV_tsubFV  z v_z a a' t
        ? lem_chgFTV_notin a a' v_z
@@ -800,30 +776,30 @@ lem_change_tvar_in_ctsubst (CConsT a1 t_a th) a a' t = case ( a == a1 ) of
                 ? lem_tchgFTV_notin a a' t_a 
                 ? lem_change_tvar_in_ctsubst th a a' (tsubFTV a1 t_a t)
 
-{-@ lem_change_var_back :: th:CSub -> { x:Vname | v_in_csubst x th }
-        -> { y:Vname | (y == x || not (in_csubst y th)) } 
+{-@ lem_change_var_back :: th:csub -> { x:vname | v_in_csubst x th }
+        -> { y:vname | (y == x || not (in_csubst y th)) } 
         -> { pf:Proof | change_varCS (change_varCS th x y) y x == th } @-}
-lem_change_var_back :: CSub -> Vname -> Vname -> Proof
+lem_change_var_back :: csub -> vname -> vname -> Proof
 lem_change_var_back CEmpty           x y               = ()
 lem_change_var_back (CCons z v_z th) x y  | ( x == z ) = ()
                                           | otherwise  = () ? lem_change_var_back th x y
 lem_change_var_back (CConsT a t_a th) x y {-| ( x == a ) = ()
                                           | otherwise  -} = () ? lem_change_var_back th x y
 
-{-@ lem_change_tvar_back :: th:CSub -> { a:Vname | tv_in_csubst a th }
-        -> { a':Vname | (a == a' || not (in_csubst a' th)) } 
+{-@ lem_change_tvar_back :: th:csub -> { a:vname | tv_in_csubst a th }
+        -> { a':vname | (a == a' || not (in_csubst a' th)) } 
         -> { pf:Proof | change_tvarCS (change_tvarCS th a a') a' a == th } @-}
-lem_change_tvar_back :: CSub -> Vname -> Vname -> Proof
+lem_change_tvar_back :: csub -> vname -> vname -> Proof
 lem_change_tvar_back CEmpty            a a'               = ()
 lem_change_tvar_back (CCons z v_z th)  a a'               = () ? lem_change_tvar_back th a a'
 lem_change_tvar_back (CConsT a1 t1 th) a a' | ( a == a1 ) = ()
                                             | otherwise   = () ? lem_change_tvar_back th a a'
 
---        -> { e:Expr | Set_sub (fv e) (bindsC th) && not (Set_mem x (fv e)) }
-{-@ lem_remove_csubst :: th:CSub -> { x:Vname | v_in_csubst x th}
-        -> { e:Expr | not (Set_mem x (fv e)) }
+--        -> { e:expr | Set_sub (fv e) (bindsC th) && not (Set_mem x (fv e)) }
+{-@ lem_remove_csubst :: th:csub -> { x:vname | v_in_csubst x th}
+        -> { e:expr | not (Set_mem x (fv e)) }
         -> { pf:Proof | csubst th e == csubst (remove_fromCS th x) e } @-}
-lem_remove_csubst :: CSub -> Vname -> Expr -> Proof
+lem_remove_csubst :: csub -> vname -> expr -> Proof
 lem_remove_csubst (CCons z v_z th) x e = case ( x == z ) of
   (True)  -> () ? lem_subFV_notin x v_z e
                   {- ? toProof ( csubst (remove_fromCS (CCons x v_z th) x) e
@@ -837,10 +813,10 @@ lem_remove_csubst (CCons z v_z th) x e = case ( x == z ) of
 lem_remove_csubst (CConsT a t_a th) x e = case ( x == a ) of
    (False) -> () ? lem_remove_csubst th x (subFTV a t_a e)
 
-{-@ lem_remove_tv_csubst :: th:CSub -> { a:Vname | tv_in_csubst a th}
-        -> { e:Expr | not (Set_mem a (ftv e)) }
+{-@ lem_remove_tv_csubst :: th:csub -> { a:vname | tv_in_csubst a th}
+        -> { e:expr | not (Set_mem a (ftv e)) }
         -> { pf:Proof | csubst th e == csubst (remove_fromCS th a) e } @-}
-lem_remove_tv_csubst :: CSub -> Vname -> Expr -> Proof
+lem_remove_tv_csubst :: csub -> vname -> expr -> Proof
 lem_remove_tv_csubst (CCons z v_z th) a e = case ( a == z ) of
   (False) -> () {- toProof ( csubst (remove_fromCS (CCons z v_z th) x) e
                    === csubst (CCons z v_z (remove_fromCS th x)) e-}
@@ -850,10 +826,10 @@ lem_remove_tv_csubst (CConsT a' t_a th) a e = case ( a == a' ) of
    (True)  -> () ? lem_subFTV_notin a t_a e
    (False) -> () ? lem_remove_tv_csubst th a (subFTV a' t_a e)
 
-{-@ lem_remove_ctsubst :: th:CSub -> { x:Vname | v_in_csubst x th}
-        -> { t:Type | not (Set_mem x (free t)) }
+{-@ lem_remove_ctsubst :: th:csub -> { x:vname | v_in_csubst x th}
+        -> { t:type | not (Set_mem x (free t)) }
         -> { pf:Proof | ctsubst th t == ctsubst (remove_fromCS th x) t } @-}
-lem_remove_ctsubst :: CSub -> Vname -> Type -> Proof
+lem_remove_ctsubst :: csub -> vname -> type -> Proof
 lem_remove_ctsubst (CCons z v_z th) x t = case ( x == z ) of
   (True)  -> () ? lem_tsubFV_notin x v_z t
           {- toProof ( ctsubst (remove_fromCS (CCons x v_z th) x) t
@@ -867,10 +843,10 @@ lem_remove_ctsubst (CCons z v_z th) x t = case ( x == z ) of
 lem_remove_ctsubst (CConsT a t_a th) x t = case ( x == a ) of
   (False) -> () ? lem_remove_ctsubst th x (tsubFTV a t_a t)
 
-{-@ lem_remove_tv_ctsubst :: th:CSub -> { a:Vname | tv_in_csubst a th}
-        -> { t:Type | not (Set_mem a (freeTV t)) }
+{-@ lem_remove_tv_ctsubst :: th:csub -> { a:vname | tv_in_csubst a th}
+        -> { t:type | not (Set_mem a (freeTV t)) }
         -> { pf:Proof | ctsubst th t == ctsubst (remove_fromCS th a) t } @-} 
-lem_remove_tv_ctsubst :: CSub -> Vname -> Type -> Proof
+lem_remove_tv_ctsubst :: csub -> vname -> type -> Proof
 lem_remove_tv_ctsubst (CCons z v_z th) a t = case ( a == z ) of
   (False) -> () ? lem_remove_tv_ctsubst th a (tsubFV z v_z t)
 lem_remove_tv_ctsubst (CConsT a' t_a th) a t = case ( a == a' ) of
